Stlc/Lemmas.v
@@ -44,9 +44,9 @@ Definition exp_mutrec :=
 
 Fixpoint close_exp_wrt_exp_rec (n1 : nat) (x1 : var) (e1 : exp) {struct e1} : exp :=
   match e1 with
+    | abs e2 => abs (close_exp_wrt_exp_rec (S n1) x1 e2)
     | var_f x2 => if (x1 == x2) then (var_b n1) else (var_f x2)
     | var_b n2 => if (lt_ge_dec n2 n1) then (var_b n2) else (var_b (S n2))
-    | abs T1 e2 => abs T1 (close_exp_wrt_exp_rec (S n1) x1 e2)
     | app e2 e3 => app (close_exp_wrt_exp_rec n1 x1 e2) (close_exp_wrt_exp_rec n1 x1 e3)
   end.
 
@@ -64,9 +64,9 @@ Fixpoint size_typ (T1 : typ) {struct T1} : nat :=
 
 Fixpoint size_exp (e1 : exp) {struct e1} : nat :=
   match e1 with
+    | abs e2 => 1 + (size_exp e2)
     | var_f x1 => 1
     | var_b n1 => 1
-    | abs T1 e2 => 1 + (size_typ T1) + (size_exp e2)
     | app e2 e3 => 1 + (size_exp e2) + (size_exp e3)
   end.
 
@@ -77,14 +77,14 @@ Fixpoint size_exp (e1 : exp) {struct e1} : nat :=
 (** These define only an upper bound, not a strict upper bound. *)
 
 Inductive degree_exp_wrt_exp : nat -> exp -> Prop :=
+  | degree_wrt_exp_abs : forall n1 e1,
+    degree_exp_wrt_exp (S n1) e1 ->
+    degree_exp_wrt_exp n1 (abs e1)
   | degree_wrt_exp_var_f : forall n1 x1,
     degree_exp_wrt_exp n1 (var_f x1)
   | degree_wrt_exp_var_b : forall n1 n2,
     lt n2 n1 ->
     degree_exp_wrt_exp n1 (var_b n2)
-  | degree_wrt_exp_abs : forall n1 T1 e1,
-    degree_exp_wrt_exp (S n1) e1 ->
-    degree_exp_wrt_exp n1 (abs T1 e1)
   | degree_wrt_exp_app : forall n1 e1 e2,
     degree_exp_wrt_exp n1 e1 ->
     degree_exp_wrt_exp n1 e2 ->
@@ -103,11 +103,11 @@ Hint Constructors degree_exp_wrt_exp : core lngen.
 (** * Local closure (version in [Set], induction principles) *)
 
 Inductive lc_set_exp : exp -> Set :=
+  | lc_set_abs : forall e1,
+    (forall x1 : var, lc_set_exp (open_exp_wrt_exp e1 (var_f x1))) ->
+    lc_set_exp (abs e1)
   | lc_set_var_f : forall x1,
     lc_set_exp (var_f x1)
-  | lc_set_abs : forall T1 e1,
-    (forall x1 : var, lc_set_exp (open_exp_wrt_exp e1 (var_f x1))) ->
-    lc_set_exp (abs T1 e1)
   | lc_set_app : forall e1 e2,
     lc_set_exp e1 ->
     lc_set_exp e2 ->
@@ -171,13 +171,18 @@ Ltac default_autorewrite ::= fail.
 
 Lemma size_typ_min_mutual :
 (forall T1, 1 <= size_typ T1).
-Proof. Admitted.
+Proof.
+apply_mutual_ind typ_mutind;
+default_simp.
+Qed.
 
 (* end hide *)
 
 Lemma size_typ_min :
 forall T1, 1 <= size_typ T1.
-Proof. Admitted.
+Proof.
+pose proof size_typ_min_mutual as H; intuition eauto.
+Qed.
 
 Hint Resolve size_typ_min : lngen.
 
@@ -185,13 +190,18 @@ Hint Resolve size_typ_min : lngen.
 
 Lemma size_exp_min_mutual :
 (forall e1, 1 <= size_exp e1).
-Proof. Admitted.
+Proof.
+apply_mutual_ind exp_mutind;
+default_simp.
+Qed.
 
 (* end hide *)
 
 Lemma size_exp_min :
 forall e1, 1 <= size_exp e1.
-Proof. Admitted.
+Proof.
+pose proof size_exp_min_mutual as H; intuition eauto.
+Qed.
 
 Hint Resolve size_exp_min : lngen.
 
@@ -200,7 +210,10 @@ Hint Resolve size_exp_min : lngen.
 Lemma size_exp_close_exp_wrt_exp_rec_mutual :
 (forall e1 x1 n1,
   size_exp (close_exp_wrt_exp_rec n1 x1 e1) = size_exp e1).
-Proof. Admitted.
+Proof.
+apply_mutual_ind exp_mutind;
+default_simp.
+Qed.
 
 (* end hide *)
 
@@ -209,7 +222,9 @@ Proof. Admitted.
 Lemma size_exp_close_exp_wrt_exp_rec :
 forall e1 x1 n1,
   size_exp (close_exp_wrt_exp_rec n1 x1 e1) = size_exp e1.
-Proof. Admitted.
+Proof.
+pose proof size_exp_close_exp_wrt_exp_rec_mutual as H; intuition eauto.
+Qed.
 
 Hint Resolve size_exp_close_exp_wrt_exp_rec : lngen.
 Hint Rewrite size_exp_close_exp_wrt_exp_rec using solve [auto] : lngen.
@@ -219,7 +234,9 @@ Hint Rewrite size_exp_close_exp_wrt_exp_rec using solve [auto] : lngen.
 Lemma size_exp_close_exp_wrt_exp :
 forall e1 x1,
   size_exp (close_exp_wrt_exp x1 e1) = size_exp e1.
-Proof. Admitted.
+Proof.
+unfold close_exp_wrt_exp; default_simp.
+Qed.
 
 Hint Resolve size_exp_close_exp_wrt_exp : lngen.
 Hint Rewrite size_exp_close_exp_wrt_exp using solve [auto] : lngen.
@@ -229,7 +246,10 @@ Hint Rewrite size_exp_close_exp_wrt_exp using solve [auto] : lngen.
 Lemma size_exp_open_exp_wrt_exp_rec_mutual :
 (forall e1 e2 n1,
   size_exp e1 <= size_exp (open_exp_wrt_exp_rec n1 e2 e1)).
-Proof. Admitted.
+Proof.
+apply_mutual_ind exp_mutind;
+default_simp.
+Qed.
 
 (* end hide *)
 
@@ -238,7 +258,9 @@ Proof. Admitted.
 Lemma size_exp_open_exp_wrt_exp_rec :
 forall e1 e2 n1,
   size_exp e1 <= size_exp (open_exp_wrt_exp_rec n1 e2 e1).
-Proof. Admitted.
+Proof.
+pose proof size_exp_open_exp_wrt_exp_rec_mutual as H; intuition eauto.
+Qed.
 
 Hint Resolve size_exp_open_exp_wrt_exp_rec : lngen.
 
@@ -247,7 +269,9 @@ Hint Resolve size_exp_open_exp_wrt_exp_rec : lngen.
 Lemma size_exp_open_exp_wrt_exp :
 forall e1 e2,
   size_exp e1 <= size_exp (open_exp_wrt_exp e1 e2).
-Proof. Admitted.
+Proof.
+unfold open_exp_wrt_exp; default_simp.
+Qed.
 
 Hint Resolve size_exp_open_exp_wrt_exp : lngen.
 
@@ -256,7 +280,10 @@ Hint Resolve size_exp_open_exp_wrt_exp : lngen.
 Lemma size_exp_open_exp_wrt_exp_rec_var_mutual :
 (forall e1 x1 n1,
   size_exp (open_exp_wrt_exp_rec n1 (var_f x1) e1) = size_exp e1).
-Proof. Admitted.
+Proof.
+apply_mutual_ind exp_mutind;
+default_simp.
+Qed.
 
 (* end hide *)
 
@@ -265,7 +292,9 @@ Proof. Admitted.
 Lemma size_exp_open_exp_wrt_exp_rec_var :
 forall e1 x1 n1,
   size_exp (open_exp_wrt_exp_rec n1 (var_f x1) e1) = size_exp e1.
-Proof. Admitted.
+Proof.
+pose proof size_exp_open_exp_wrt_exp_rec_var_mutual as H; intuition eauto.
+Qed.
 
 Hint Resolve size_exp_open_exp_wrt_exp_rec_var : lngen.
 Hint Rewrite size_exp_open_exp_wrt_exp_rec_var using solve [auto] : lngen.
@@ -275,7 +304,9 @@ Hint Rewrite size_exp_open_exp_wrt_exp_rec_var using solve [auto] : lngen.
 Lemma size_exp_open_exp_wrt_exp_var :
 forall e1 x1,
   size_exp (open_exp_wrt_exp e1 (var_f x1)) = size_exp e1.
-Proof. Admitted.
+Proof.
+unfold open_exp_wrt_exp; default_simp.
+Qed.
 
 Hint Resolve size_exp_open_exp_wrt_exp_var : lngen.
 Hint Rewrite size_exp_open_exp_wrt_exp_var using solve [auto] : lngen.
@@ -293,7 +324,10 @@ Lemma degree_exp_wrt_exp_S_mutual :
 (forall n1 e1,
   degree_exp_wrt_exp n1 e1 ->
   degree_exp_wrt_exp (S n1) e1).
-Proof. Admitted.
+Proof.
+apply_mutual_ind degree_exp_wrt_exp_mutind;
+default_simp.
+Qed.
 
 (* end hide *)
 
@@ -301,7 +335,9 @@ Lemma degree_exp_wrt_exp_S :
 forall n1 e1,
   degree_exp_wrt_exp n1 e1 ->
   degree_exp_wrt_exp (S n1) e1.
-Proof. Admitted.
+Proof.
+pose proof degree_exp_wrt_exp_S_mutual as H; intuition eauto.
+Qed.
 
 Hint Resolve degree_exp_wrt_exp_S : lngen.
 
@@ -309,7 +345,9 @@ Lemma degree_exp_wrt_exp_O :
 forall n1 e1,
   degree_exp_wrt_exp O e1 ->
   degree_exp_wrt_exp n1 e1.
-Proof. Admitted.
+Proof.
+induction n1; default_simp.
+Qed.
 
 Hint Resolve degree_exp_wrt_exp_O : lngen.
 
@@ -319,7 +357,10 @@ Lemma degree_exp_wrt_exp_close_exp_wrt_exp_rec_mutual :
 (forall e1 x1 n1,
   degree_exp_wrt_exp n1 e1 ->
   degree_exp_wrt_exp (S n1) (close_exp_wrt_exp_rec n1 x1 e1)).
-Proof. Admitted.
+Proof.
+apply_mutual_ind exp_mutind;
+default_simp.
+Qed.
 
 (* end hide *)
 
@@ -329,7 +370,9 @@ Lemma degree_exp_wrt_exp_close_exp_wrt_exp_rec :
 forall e1 x1 n1,
   degree_exp_wrt_exp n1 e1 ->
   degree_exp_wrt_exp (S n1) (close_exp_wrt_exp_rec n1 x1 e1).
-Proof. Admitted.
+Proof.
+pose proof degree_exp_wrt_exp_close_exp_wrt_exp_rec_mutual as H; intuition eauto.
+Qed.
 
 Hint Resolve degree_exp_wrt_exp_close_exp_wrt_exp_rec : lngen.
 
@@ -339,7 +382,9 @@ Lemma degree_exp_wrt_exp_close_exp_wrt_exp :
 forall e1 x1,
   degree_exp_wrt_exp 0 e1 ->
   degree_exp_wrt_exp 1 (close_exp_wrt_exp x1 e1).
-Proof. Admitted.
+Proof.
+unfold close_exp_wrt_exp; default_simp.
+Qed.
 
 Hint Resolve degree_exp_wrt_exp_close_exp_wrt_exp : lngen.
 
@@ -349,7 +394,10 @@ Lemma degree_exp_wrt_exp_close_exp_wrt_exp_rec_inv_mutual :
 (forall e1 x1 n1,
   degree_exp_wrt_exp (S n1) (close_exp_wrt_exp_rec n1 x1 e1) ->
   degree_exp_wrt_exp n1 e1).
-Proof. Admitted.
+Proof.
+apply_mutual_ind exp_mutind;
+default_simp; eauto with lngen.
+Qed.
 
 (* end hide *)
 
@@ -359,7 +407,9 @@ Lemma degree_exp_wrt_exp_close_exp_wrt_exp_rec_inv :
 forall e1 x1 n1,
   degree_exp_wrt_exp (S n1) (close_exp_wrt_exp_rec n1 x1 e1) ->
   degree_exp_wrt_exp n1 e1.
-Proof. Admitted.
+Proof.
+pose proof degree_exp_wrt_exp_close_exp_wrt_exp_rec_inv_mutual as H; intuition eauto.
+Qed.
 
 Hint Immediate degree_exp_wrt_exp_close_exp_wrt_exp_rec_inv : lngen.
 
@@ -369,7 +419,9 @@ Lemma degree_exp_wrt_exp_close_exp_wrt_exp_inv :
 forall e1 x1,
   degree_exp_wrt_exp 1 (close_exp_wrt_exp x1 e1) ->
   degree_exp_wrt_exp 0 e1.
-Proof. Admitted.
+Proof.
+unfold close_exp_wrt_exp; eauto with lngen.
+Qed.
 
 Hint Immediate degree_exp_wrt_exp_close_exp_wrt_exp_inv : lngen.
 
@@ -380,7 +432,10 @@ Lemma degree_exp_wrt_exp_open_exp_wrt_exp_rec_mutual :
   degree_exp_wrt_exp (S n1) e1 ->
   degree_exp_wrt_exp n1 e2 ->
   degree_exp_wrt_exp n1 (open_exp_wrt_exp_rec n1 e2 e1)).
-Proof. Admitted.
+Proof.
+apply_mutual_ind exp_mutind;
+default_simp.
+Qed.
 
 (* end hide *)
 
@@ -391,7 +446,9 @@ forall e1 e2 n1,
   degree_exp_wrt_exp (S n1) e1 ->
   degree_exp_wrt_exp n1 e2 ->
   degree_exp_wrt_exp n1 (open_exp_wrt_exp_rec n1 e2 e1).
-Proof. Admitted.
+Proof.
+pose proof degree_exp_wrt_exp_open_exp_wrt_exp_rec_mutual as H; intuition eauto.
+Qed.
 
 Hint Resolve degree_exp_wrt_exp_open_exp_wrt_exp_rec : lngen.
 
@@ -402,7 +459,9 @@ forall e1 e2,
   degree_exp_wrt_exp 1 e1 ->
   degree_exp_wrt_exp 0 e2 ->
   degree_exp_wrt_exp 0 (open_exp_wrt_exp e1 e2).
-Proof. Admitted.
+Proof.
+unfold open_exp_wrt_exp; default_simp.
+Qed.
 
 Hint Resolve degree_exp_wrt_exp_open_exp_wrt_exp : lngen.
 
@@ -412,7 +471,10 @@ Lemma degree_exp_wrt_exp_open_exp_wrt_exp_rec_inv_mutual :
 (forall e1 e2 n1,
   degree_exp_wrt_exp n1 (open_exp_wrt_exp_rec n1 e2 e1) ->
   degree_exp_wrt_exp (S n1) e1).
-Proof. Admitted.
+Proof.
+apply_mutual_ind exp_mutind;
+default_simp; eauto with lngen.
+Qed.
 
 (* end hide *)
 
@@ -422,7 +484,9 @@ Lemma degree_exp_wrt_exp_open_exp_wrt_exp_rec_inv :
 forall e1 e2 n1,
   degree_exp_wrt_exp n1 (open_exp_wrt_exp_rec n1 e2 e1) ->
   degree_exp_wrt_exp (S n1) e1.
-Proof. Admitted.
+Proof.
+pose proof degree_exp_wrt_exp_open_exp_wrt_exp_rec_inv_mutual as H; intuition eauto.
+Qed.
 
 Hint Immediate degree_exp_wrt_exp_open_exp_wrt_exp_rec_inv : lngen.
 
@@ -432,7 +496,9 @@ Lemma degree_exp_wrt_exp_open_exp_wrt_exp_inv :
 forall e1 e2,
   degree_exp_wrt_exp 0 (open_exp_wrt_exp e1 e2) ->
   degree_exp_wrt_exp 1 e1.
-Proof. Admitted.
+Proof.
+unfold open_exp_wrt_exp; eauto with lngen.
+Qed.
 
 Hint Immediate degree_exp_wrt_exp_open_exp_wrt_exp_inv : lngen.
 
@@ -449,7 +515,13 @@ Lemma close_exp_wrt_exp_rec_inj_mutual :
 (forall e1 e2 x1 n1,
   close_exp_wrt_exp_rec n1 x1 e1 = close_exp_wrt_exp_rec n1 x1 e2 ->
   e1 = e2).
-Proof. Admitted.
+Proof.
+apply_mutual_ind exp_mutind;
+intros; match goal with
+          | |- _ = ?term => destruct term
+        end;
+default_simp; eauto with lngen.
+Qed.
 
 (* end hide *)
 
@@ -459,7 +531,9 @@ Lemma close_exp_wrt_exp_rec_inj :
 forall e1 e2 x1 n1,
   close_exp_wrt_exp_rec n1 x1 e1 = close_exp_wrt_exp_rec n1 x1 e2 ->
   e1 = e2.
-Proof. Admitted.
+Proof.
+pose proof close_exp_wrt_exp_rec_inj_mutual as H; intuition eauto.
+Qed.
 
 Hint Immediate close_exp_wrt_exp_rec_inj : lngen.
 
@@ -469,7 +543,9 @@ Lemma close_exp_wrt_exp_inj :
 forall e1 e2 x1,
   close_exp_wrt_exp x1 e1 = close_exp_wrt_exp x1 e2 ->
   e1 = e2.
-Proof. Admitted.
+Proof.
+unfold close_exp_wrt_exp; eauto with lngen.
+Qed.
 
 Hint Immediate close_exp_wrt_exp_inj : lngen.
 
@@ -479,7 +555,10 @@ Lemma close_exp_wrt_exp_rec_open_exp_wrt_exp_rec_mutual :
 (forall e1 x1 n1,
   x1 `notin` fv_exp e1 ->
   close_exp_wrt_exp_rec n1 x1 (open_exp_wrt_exp_rec n1 (var_f x1) e1) = e1).
-Proof. Admitted.
+Proof.
+apply_mutual_ind exp_mutind;
+default_simp.
+Qed.
 
 (* end hide *)
 
@@ -489,7 +568,9 @@ Lemma close_exp_wrt_exp_rec_open_exp_wrt_exp_rec :
 forall e1 x1 n1,
   x1 `notin` fv_exp e1 ->
   close_exp_wrt_exp_rec n1 x1 (open_exp_wrt_exp_rec n1 (var_f x1) e1) = e1.
-Proof. Admitted.
+Proof.
+pose proof close_exp_wrt_exp_rec_open_exp_wrt_exp_rec_mutual as H; intuition eauto.
+Qed.
 
 Hint Resolve close_exp_wrt_exp_rec_open_exp_wrt_exp_rec : lngen.
 Hint Rewrite close_exp_wrt_exp_rec_open_exp_wrt_exp_rec using solve [auto] : lngen.
@@ -500,7 +581,9 @@ Lemma close_exp_wrt_exp_open_exp_wrt_exp :
 forall e1 x1,
   x1 `notin` fv_exp e1 ->
   close_exp_wrt_exp x1 (open_exp_wrt_exp e1 (var_f x1)) = e1.
-Proof. Admitted.
+Proof.
+unfold close_exp_wrt_exp; unfold open_exp_wrt_exp; default_simp.
+Qed.
 
 Hint Resolve close_exp_wrt_exp_open_exp_wrt_exp : lngen.
 Hint Rewrite close_exp_wrt_exp_open_exp_wrt_exp using solve [auto] : lngen.
@@ -510,7 +593,10 @@ Hint Rewrite close_exp_wrt_exp_open_exp_wrt_exp using solve [auto] : lngen.
 Lemma open_exp_wrt_exp_rec_close_exp_wrt_exp_rec_mutual :
 (forall e1 x1 n1,
   open_exp_wrt_exp_rec n1 (var_f x1) (close_exp_wrt_exp_rec n1 x1 e1) = e1).
-Proof. Admitted.
+Proof.
+apply_mutual_ind exp_mutind;
+default_simp.
+Qed.
 
 (* end hide *)
 
@@ -519,7 +605,9 @@ Proof. Admitted.
 Lemma open_exp_wrt_exp_rec_close_exp_wrt_exp_rec :
 forall e1 x1 n1,
   open_exp_wrt_exp_rec n1 (var_f x1) (close_exp_wrt_exp_rec n1 x1 e1) = e1.
-Proof. Admitted.
+Proof.
+pose proof open_exp_wrt_exp_rec_close_exp_wrt_exp_rec_mutual as H; intuition eauto.
+Qed.
 
 Hint Resolve open_exp_wrt_exp_rec_close_exp_wrt_exp_rec : lngen.
 Hint Rewrite open_exp_wrt_exp_rec_close_exp_wrt_exp_rec using solve [auto] : lngen.
@@ -529,7 +617,9 @@ Hint Rewrite open_exp_wrt_exp_rec_close_exp_wrt_exp_rec using solve [auto] : lng
 Lemma open_exp_wrt_exp_close_exp_wrt_exp :
 forall e1 x1,
   open_exp_wrt_exp (close_exp_wrt_exp x1 e1) (var_f x1) = e1.
-Proof. Admitted.
+Proof.
+unfold close_exp_wrt_exp; unfold open_exp_wrt_exp; default_simp.
+Qed.
 
 Hint Resolve open_exp_wrt_exp_close_exp_wrt_exp : lngen.
 Hint Rewrite open_exp_wrt_exp_close_exp_wrt_exp using solve [auto] : lngen.
@@ -542,7 +632,13 @@ Lemma open_exp_wrt_exp_rec_inj_mutual :
   x1 `notin` fv_exp e1 ->
   open_exp_wrt_exp_rec n1 (var_f x1) e2 = open_exp_wrt_exp_rec n1 (var_f x1) e1 ->
   e2 = e1).
-Proof. Admitted.
+Proof.
+apply_mutual_ind exp_mutind;
+intros; match goal with
+          | |- _ = ?term => destruct term
+        end;
+default_simp; eauto with lngen.
+Qed.
 
 (* end hide *)
 
@@ -554,7 +650,9 @@ forall e2 e1 x1 n1,
   x1 `notin` fv_exp e1 ->
   open_exp_wrt_exp_rec n1 (var_f x1) e2 = open_exp_wrt_exp_rec n1 (var_f x1) e1 ->
   e2 = e1.
-Proof. Admitted.
+Proof.
+pose proof open_exp_wrt_exp_rec_inj_mutual as H; intuition eauto.
+Qed.
 
 Hint Immediate open_exp_wrt_exp_rec_inj : lngen.
 
@@ -566,7 +664,9 @@ forall e2 e1 x1,
   x1 `notin` fv_exp e1 ->
   open_exp_wrt_exp e2 (var_f x1) = open_exp_wrt_exp e1 (var_f x1) ->
   e2 = e1.
-Proof. Admitted.
+Proof.
+unfold open_exp_wrt_exp; eauto with lngen.
+Qed.
 
 Hint Immediate open_exp_wrt_exp_inj : lngen.
 
@@ -583,7 +683,15 @@ Lemma degree_exp_wrt_exp_of_lc_exp_mutual :
 (forall e1,
   lc_exp e1 ->
   degree_exp_wrt_exp 0 e1).
-Proof. Admitted.
+Proof.
+apply_mutual_ind lc_exp_mutind;
+intros;
+let x1 := fresh "x1" in pick_fresh x1;
+repeat (match goal with
+          | H1 : _, H2 : _ |- _ => specialize H1 with H2
+        end);
+default_simp; eauto with lngen.
+Qed.
 
 (* end hide *)
 
@@ -591,7 +699,9 @@ Lemma degree_exp_wrt_exp_of_lc_exp :
 forall e1,
   lc_exp e1 ->
   degree_exp_wrt_exp 0 e1.
-Proof. Admitted.
+Proof.
+pose proof degree_exp_wrt_exp_of_lc_exp_mutual as H; intuition eauto.
+Qed.
 
 Hint Resolve degree_exp_wrt_exp_of_lc_exp : lngen.
 
@@ -603,7 +713,22 @@ forall i1,
   size_exp e1 = i1 ->
   degree_exp_wrt_exp 0 e1 ->
   lc_exp e1).
-Proof. Admitted.
+Proof.
+intros i1; pattern i1; apply lt_wf_rec;
+clear i1; intros i1 H1;
+apply_mutual_ind exp_mutind;
+default_simp;
+(* non-trivial cases *)
+constructor; default_simp; eapply_first_lt_hyp;
+(* instantiate the size *)
+match goal with
+  | |- _ = _ => reflexivity
+  | _ => idtac
+end;
+instantiate;
+(* everything should be easy now *)
+default_simp.
+Qed.
 
 (* end hide *)
 
@@ -611,7 +736,11 @@ Lemma lc_exp_of_degree :
 forall e1,
   degree_exp_wrt_exp 0 e1 ->
   lc_exp e1.
-Proof. Admitted.
+Proof.
+intros e1; intros;
+pose proof (lc_exp_of_degree_size_mutual (size_exp e1));
+intuition eauto.
+Qed.
 
 Hint Resolve lc_exp_of_degree : lngen.
 
@@ -628,12 +757,14 @@ Ltac exp_lc_exists_tac :=
           end).
 
 Lemma lc_abs_exists :
-forall x1 T1 e1,
+forall x1 e1,
   lc_exp (open_exp_wrt_exp e1 (var_f x1)) ->
-  lc_exp (abs T1 e1).
-Proof. Admitted.
+  lc_exp (abs e1).
+Proof.
+intros; exp_lc_exists_tac; eauto with lngen.
+Qed.
 
-Hint Extern 1 (lc_exp (abs _ _)) =>
+Hint Extern 1 (lc_exp (abs _)) =>
   let x1 := fresh in
   pick_fresh x1;
   apply (lc_abs_exists x1).
@@ -643,29 +774,47 @@ forall e1 e2,
   body_exp_wrt_exp e1 ->
   lc_exp e2 ->
   lc_exp (open_exp_wrt_exp e1 e2).
-Proof. Admitted.
+Proof.
+unfold body_exp_wrt_exp;
+default_simp;
+let x1 := fresh "x" in
+pick_fresh x1;
+specialize_all x1;
+exp_lc_exists_tac;
+eauto with lngen.
+Qed.
 
 Hint Resolve lc_body_exp_wrt_exp : lngen.
 
-Lemma lc_body_abs_2 :
-forall T1 e1,
-  lc_exp (abs T1 e1) ->
+Lemma lc_body_abs_1 :
+forall e1,
+  lc_exp (abs e1) ->
   body_exp_wrt_exp e1.
-Proof. Admitted.
+Proof.
+default_simp.
+Qed.
 
-Hint Resolve lc_body_abs_2 : lngen.
+Hint Resolve lc_body_abs_1 : lngen.
 
 (* begin hide *)
 
 Lemma lc_exp_unique_mutual :
 (forall e1 (proof2 proof3 : lc_exp e1), proof2 = proof3).
-Proof. Admitted.
+Proof.
+apply_mutual_ind lc_exp_mutind;
+intros;
+let proof1 := fresh "proof1" in
+rename_last_into proof1; dependent destruction proof1;
+f_equal; default_simp; auto using @functional_extensionality_dep with lngen.
+Qed.
 
 (* end hide *)
 
 Lemma lc_exp_unique :
 forall e1 (proof2 proof3 : lc_exp e1), proof2 = proof3.
-Proof. Admitted.
+Proof.
+pose proof lc_exp_unique_mutual as H; intuition eauto.
+Qed.
 
 Hint Resolve lc_exp_unique : lngen.
 
@@ -673,13 +822,18 @@ Hint Resolve lc_exp_unique : lngen.
 
 Lemma lc_exp_of_lc_set_exp_mutual :
 (forall e1, lc_set_exp e1 -> lc_exp e1).
-Proof. Admitted.
+Proof.
+apply_mutual_ind lc_set_exp_mutind;
+default_simp.
+Qed.
 
 (* end hide *)
 
 Lemma lc_exp_of_lc_set_exp :
 forall e1, lc_set_exp e1 -> lc_exp e1.
-Proof. Admitted.
+Proof.
+pose proof lc_exp_of_lc_set_exp_mutual as H; intuition eauto.
+Qed.
 
 Hint Resolve lc_exp_of_lc_set_exp : lngen.
 
@@ -691,7 +845,25 @@ forall i1,
   size_exp e1 = i1 ->
   lc_exp e1 ->
   lc_set_exp e1).
-Proof. Admitted.
+Proof.
+intros i1; pattern i1; apply lt_wf_rec;
+clear i1; intros i1 H1;
+apply_mutual_ind exp_mutrec;
+default_simp;
+try solve [assert False by default_simp; tauto];
+(* non-trivial cases *)
+constructor; default_simp;
+try first [apply lc_set_exp_of_lc_exp];
+default_simp; eapply_first_lt_hyp;
+(* instantiate the size *)
+match goal with
+  | |- _ = _ => reflexivity
+  | _ => idtac
+end;
+instantiate;
+(* everything should be easy now *)
+default_simp.
+Qed.
 
 (* end hide *)
 
@@ -699,7 +871,11 @@ Lemma lc_set_exp_of_lc_exp :
 forall e1,
   lc_exp e1 ->
   lc_set_exp e1.
-Proof. Admitted.
+Proof.
+intros e1; intros;
+pose proof (lc_set_exp_of_lc_exp_size_mutual (size_exp e1));
+intuition eauto.
+Qed.
 
 Hint Resolve lc_set_exp_of_lc_exp : lngen.
 
@@ -717,7 +893,10 @@ Lemma close_exp_wrt_exp_rec_degree_exp_wrt_exp_mutual :
   degree_exp_wrt_exp n1 e1 ->
   x1 `notin` fv_exp e1 ->
   close_exp_wrt_exp_rec n1 x1 e1 = e1).
-Proof. Admitted.
+Proof.
+apply_mutual_ind exp_mutind;
+default_simp.
+Qed.
 
 (* end hide *)
 
@@ -728,7 +907,9 @@ forall e1 x1 n1,
   degree_exp_wrt_exp n1 e1 ->
   x1 `notin` fv_exp e1 ->
   close_exp_wrt_exp_rec n1 x1 e1 = e1.
-Proof. Admitted.
+Proof.
+pose proof close_exp_wrt_exp_rec_degree_exp_wrt_exp_mutual as H; intuition eauto.
+Qed.
 
 Hint Resolve close_exp_wrt_exp_rec_degree_exp_wrt_exp : lngen.
 Hint Rewrite close_exp_wrt_exp_rec_degree_exp_wrt_exp using solve [auto] : lngen.
@@ -740,7 +921,9 @@ forall e1 x1,
   lc_exp e1 ->
   x1 `notin` fv_exp e1 ->
   close_exp_wrt_exp x1 e1 = e1.
-Proof. Admitted.
+Proof.
+unfold close_exp_wrt_exp; default_simp.
+Qed.
 
 Hint Resolve close_exp_wrt_exp_lc_exp : lngen.
 Hint Rewrite close_exp_wrt_exp_lc_exp using solve [auto] : lngen.
@@ -751,7 +934,10 @@ Lemma open_exp_wrt_exp_rec_degree_exp_wrt_exp_mutual :
 (forall e2 e1 n1,
   degree_exp_wrt_exp n1 e2 ->
   open_exp_wrt_exp_rec n1 e1 e2 = e2).
-Proof. Admitted.
+Proof.
+apply_mutual_ind exp_mutind;
+default_simp.
+Qed.
 
 (* end hide *)
 
@@ -761,7 +947,9 @@ Lemma open_exp_wrt_exp_rec_degree_exp_wrt_exp :
 forall e2 e1 n1,
   degree_exp_wrt_exp n1 e2 ->
   open_exp_wrt_exp_rec n1 e1 e2 = e2.
-Proof. Admitted.
+Proof.
+pose proof open_exp_wrt_exp_rec_degree_exp_wrt_exp_mutual as H; intuition eauto.
+Qed.
 
 Hint Resolve open_exp_wrt_exp_rec_degree_exp_wrt_exp : lngen.
 Hint Rewrite open_exp_wrt_exp_rec_degree_exp_wrt_exp using solve [auto] : lngen.
@@ -772,7 +960,9 @@ Lemma open_exp_wrt_exp_lc_exp :
 forall e2 e1,
   lc_exp e2 ->
   open_exp_wrt_exp e2 e1 = e2.
-Proof. Admitted.
+Proof.
+unfold open_exp_wrt_exp; default_simp.
+Qed.
 
 Hint Resolve open_exp_wrt_exp_lc_exp : lngen.
 Hint Rewrite open_exp_wrt_exp_lc_exp using solve [auto] : lngen.
@@ -789,7 +979,10 @@ Ltac default_autorewrite ::= autorewrite with lngen.
 Lemma fv_exp_close_exp_wrt_exp_rec_mutual :
 (forall e1 x1 n1,
   fv_exp (close_exp_wrt_exp_rec n1 x1 e1) [=] remove x1 (fv_exp e1)).
-Proof. Admitted.
+Proof.
+apply_mutual_ind exp_mutind;
+default_simp; fsetdec.
+Qed.
 
 (* end hide *)
 
@@ -798,7 +991,9 @@ Proof. Admitted.
 Lemma fv_exp_close_exp_wrt_exp_rec :
 forall e1 x1 n1,
   fv_exp (close_exp_wrt_exp_rec n1 x1 e1) [=] remove x1 (fv_exp e1).
-Proof. Admitted.
+Proof.
+pose proof fv_exp_close_exp_wrt_exp_rec_mutual as H; intuition eauto.
+Qed.
 
 Hint Resolve fv_exp_close_exp_wrt_exp_rec : lngen.
 Hint Rewrite fv_exp_close_exp_wrt_exp_rec using solve [auto] : lngen.
@@ -808,7 +1003,9 @@ Hint Rewrite fv_exp_close_exp_wrt_exp_rec using solve [auto] : lngen.
 Lemma fv_exp_close_exp_wrt_exp :
 forall e1 x1,
   fv_exp (close_exp_wrt_exp x1 e1) [=] remove x1 (fv_exp e1).
-Proof. Admitted.
+Proof.
+unfold close_exp_wrt_exp; default_simp.
+Qed.
 
 Hint Resolve fv_exp_close_exp_wrt_exp : lngen.
 Hint Rewrite fv_exp_close_exp_wrt_exp using solve [auto] : lngen.
@@ -818,7 +1015,10 @@ Hint Rewrite fv_exp_close_exp_wrt_exp using solve [auto] : lngen.
 Lemma fv_exp_open_exp_wrt_exp_rec_lower_mutual :
 (forall e1 e2 n1,
   fv_exp e1 [<=] fv_exp (open_exp_wrt_exp_rec n1 e2 e1)).
-Proof. Admitted.
+Proof.
+apply_mutual_ind exp_mutind;
+default_simp; fsetdec.
+Qed.
 
 (* end hide *)
 
@@ -827,7 +1027,9 @@ Proof. Admitted.
 Lemma fv_exp_open_exp_wrt_exp_rec_lower :
 forall e1 e2 n1,
   fv_exp e1 [<=] fv_exp (open_exp_wrt_exp_rec n1 e2 e1).
-Proof. Admitted.
+Proof.
+pose proof fv_exp_open_exp_wrt_exp_rec_lower_mutual as H; intuition eauto.
+Qed.
 
 Hint Resolve fv_exp_open_exp_wrt_exp_rec_lower : lngen.
 
@@ -836,7 +1038,9 @@ Hint Resolve fv_exp_open_exp_wrt_exp_rec_lower : lngen.
 Lemma fv_exp_open_exp_wrt_exp_lower :
 forall e1 e2,
   fv_exp e1 [<=] fv_exp (open_exp_wrt_exp e1 e2).
-Proof. Admitted.
+Proof.
+unfold open_exp_wrt_exp; default_simp.
+Qed.
 
 Hint Resolve fv_exp_open_exp_wrt_exp_lower : lngen.
 
@@ -845,7 +1049,10 @@ Hint Resolve fv_exp_open_exp_wrt_exp_lower : lngen.
 Lemma fv_exp_open_exp_wrt_exp_rec_upper_mutual :
 (forall e1 e2 n1,
   fv_exp (open_exp_wrt_exp_rec n1 e2 e1) [<=] fv_exp e2 `union` fv_exp e1).
-Proof. Admitted.
+Proof.
+apply_mutual_ind exp_mutind;
+default_simp; fsetdec.
+Qed.
 
 (* end hide *)
 
@@ -854,7 +1061,9 @@ Proof. Admitted.
 Lemma fv_exp_open_exp_wrt_exp_rec_upper :
 forall e1 e2 n1,
   fv_exp (open_exp_wrt_exp_rec n1 e2 e1) [<=] fv_exp e2 `union` fv_exp e1.
-Proof. Admitted.
+Proof.
+pose proof fv_exp_open_exp_wrt_exp_rec_upper_mutual as H; intuition eauto.
+Qed.
 
 Hint Resolve fv_exp_open_exp_wrt_exp_rec_upper : lngen.
 
@@ -863,7 +1072,9 @@ Hint Resolve fv_exp_open_exp_wrt_exp_rec_upper : lngen.
 Lemma fv_exp_open_exp_wrt_exp_upper :
 forall e1 e2,
   fv_exp (open_exp_wrt_exp e1 e2) [<=] fv_exp e2 `union` fv_exp e1.
-Proof. Admitted.
+Proof.
+unfold open_exp_wrt_exp; default_simp.
+Qed.
 
 Hint Resolve fv_exp_open_exp_wrt_exp_upper : lngen.
 
@@ -873,7 +1084,10 @@ Lemma fv_exp_subst_exp_fresh_mutual :
 (forall e1 e2 x1,
   x1 `notin` fv_exp e1 ->
   fv_exp (subst_exp e2 x1 e1) [=] fv_exp e1).
-Proof. Admitted.
+Proof.
+apply_mutual_ind exp_mutind;
+default_simp; fsetdec.
+Qed.
 
 (* end hide *)
 
@@ -881,7 +1095,9 @@ Lemma fv_exp_subst_exp_fresh :
 forall e1 e2 x1,
   x1 `notin` fv_exp e1 ->
   fv_exp (subst_exp e2 x1 e1) [=] fv_exp e1.
-Proof. Admitted.
+Proof.
+pose proof fv_exp_subst_exp_fresh_mutual as H; intuition eauto.
+Qed.
 
 Hint Resolve fv_exp_subst_exp_fresh : lngen.
 Hint Rewrite fv_exp_subst_exp_fresh using solve [auto] : lngen.
@@ -891,14 +1107,19 @@ Hint Rewrite fv_exp_subst_exp_fresh using solve [auto] : lngen.
 Lemma fv_exp_subst_exp_lower_mutual :
 (forall e1 e2 x1,
   remove x1 (fv_exp e1) [<=] fv_exp (subst_exp e2 x1 e1)).
-Proof. Admitted.
+Proof.
+apply_mutual_ind exp_mutind;
+default_simp; fsetdec.
+Qed.
 
 (* end hide *)
 
 Lemma fv_exp_subst_exp_lower :
 forall e1 e2 x1,
   remove x1 (fv_exp e1) [<=] fv_exp (subst_exp e2 x1 e1).
-Proof. Admitted.
+Proof.
+pose proof fv_exp_subst_exp_lower_mutual as H; intuition eauto.
+Qed.
 
 Hint Resolve fv_exp_subst_exp_lower : lngen.
 
@@ -909,7 +1130,10 @@ Lemma fv_exp_subst_exp_notin_mutual :
   x2 `notin` fv_exp e1 ->
   x2 `notin` fv_exp e2 ->
   x2 `notin` fv_exp (subst_exp e2 x1 e1)).
-Proof. Admitted.
+Proof.
+apply_mutual_ind exp_mutind;
+default_simp; fsetdec.
+Qed.
 
 (* end hide *)
 
@@ -918,7 +1142,9 @@ forall e1 e2 x1 x2,
   x2 `notin` fv_exp e1 ->
   x2 `notin` fv_exp e2 ->
   x2 `notin` fv_exp (subst_exp e2 x1 e1).
-Proof. Admitted.
+Proof.
+pose proof fv_exp_subst_exp_notin_mutual as H; intuition eauto.
+Qed.
 
 Hint Resolve fv_exp_subst_exp_notin : lngen.
 
@@ -927,14 +1153,19 @@ Hint Resolve fv_exp_subst_exp_notin : lngen.
 Lemma fv_exp_subst_exp_upper_mutual :
 (forall e1 e2 x1,
   fv_exp (subst_exp e2 x1 e1) [<=] fv_exp e2 `union` remove x1 (fv_exp e1)).
-Proof. Admitted.
+Proof.
+apply_mutual_ind exp_mutind;
+default_simp; fsetdec.
+Qed.
 
 (* end hide *)
 
 Lemma fv_exp_subst_exp_upper :
 forall e1 e2 x1,
   fv_exp (subst_exp e2 x1 e1) [<=] fv_exp e2 `union` remove x1 (fv_exp e1).
-Proof. Admitted.
+Proof.
+pose proof fv_exp_subst_exp_upper_mutual as H; intuition eauto.
+Qed.
 
 Hint Resolve fv_exp_subst_exp_upper : lngen.
 
@@ -953,7 +1184,10 @@ Lemma subst_exp_close_exp_wrt_exp_rec_mutual :
   x1 <> x2 ->
   x2 `notin` fv_exp e1 ->
   subst_exp e1 x1 (close_exp_wrt_exp_rec n1 x2 e2) = close_exp_wrt_exp_rec n1 x2 (subst_exp e1 x1 e2)).
-Proof. Admitted.
+Proof.
+apply_mutual_ind exp_mutind;
+default_simp.
+Qed.
 
 (* end hide *)
 
@@ -963,7 +1197,9 @@ forall e2 e1 x1 x2 n1,
   x1 <> x2 ->
   x2 `notin` fv_exp e1 ->
   subst_exp e1 x1 (close_exp_wrt_exp_rec n1 x2 e2) = close_exp_wrt_exp_rec n1 x2 (subst_exp e1 x1 e2).
-Proof. Admitted.
+Proof.
+pose proof subst_exp_close_exp_wrt_exp_rec_mutual as H; intuition eauto.
+Qed.
 
 Hint Resolve subst_exp_close_exp_wrt_exp_rec : lngen.
 
@@ -972,7 +1208,9 @@ forall e2 e1 x1 x2,
   lc_exp e1 ->  x1 <> x2 ->
   x2 `notin` fv_exp e1 ->
   subst_exp e1 x1 (close_exp_wrt_exp x2 e2) = close_exp_wrt_exp x2 (subst_exp e1 x1 e2).
-Proof. Admitted.
+Proof.
+unfold close_exp_wrt_exp; default_simp.
+Qed.
 
 Hint Resolve subst_exp_close_exp_wrt_exp : lngen.
 
@@ -983,7 +1221,10 @@ Lemma subst_exp_degree_exp_wrt_exp_mutual :
   degree_exp_wrt_exp n1 e1 ->
   degree_exp_wrt_exp n1 e2 ->
   degree_exp_wrt_exp n1 (subst_exp e2 x1 e1)).
-Proof. Admitted.
+Proof.
+apply_mutual_ind exp_mutind;
+default_simp.
+Qed.
 
 (* end hide *)
 
@@ -992,7 +1233,9 @@ forall e1 e2 x1 n1,
   degree_exp_wrt_exp n1 e1 ->
   degree_exp_wrt_exp n1 e2 ->
   degree_exp_wrt_exp n1 (subst_exp e2 x1 e1).
-Proof. Admitted.
+Proof.
+pose proof subst_exp_degree_exp_wrt_exp_mutual as H; intuition eauto.
+Qed.
 
 Hint Resolve subst_exp_degree_exp_wrt_exp : lngen.
 
@@ -1002,7 +1245,10 @@ Lemma subst_exp_fresh_eq_mutual :
 (forall e2 e1 x1,
   x1 `notin` fv_exp e2 ->
   subst_exp e1 x1 e2 = e2).
-Proof. Admitted.
+Proof.
+apply_mutual_ind exp_mutind;
+default_simp.
+Qed.
 
 (* end hide *)
 
@@ -1010,7 +1256,9 @@ Lemma subst_exp_fresh_eq :
 forall e2 e1 x1,
   x1 `notin` fv_exp e2 ->
   subst_exp e1 x1 e2 = e2.
-Proof. Admitted.
+Proof.
+pose proof subst_exp_fresh_eq_mutual as H; intuition eauto.
+Qed.
 
 Hint Resolve subst_exp_fresh_eq : lngen.
 Hint Rewrite subst_exp_fresh_eq using solve [auto] : lngen.
@@ -1021,7 +1269,10 @@ Lemma subst_exp_fresh_same_mutual :
 (forall e2 e1 x1,
   x1 `notin` fv_exp e1 ->
   x1 `notin` fv_exp (subst_exp e1 x1 e2)).
-Proof. Admitted.
+Proof.
+apply_mutual_ind exp_mutind;
+default_simp.
+Qed.
 
 (* end hide *)
 
@@ -1029,7 +1280,9 @@ Lemma subst_exp_fresh_same :
 forall e2 e1 x1,
   x1 `notin` fv_exp e1 ->
   x1 `notin` fv_exp (subst_exp e1 x1 e2).
-Proof. Admitted.
+Proof.
+pose proof subst_exp_fresh_same_mutual as H; intuition eauto.
+Qed.
 
 Hint Resolve subst_exp_fresh_same : lngen.
 
@@ -1040,7 +1293,10 @@ Lemma subst_exp_fresh_mutual :
   x1 `notin` fv_exp e2 ->
   x1 `notin` fv_exp e1 ->
   x1 `notin` fv_exp (subst_exp e1 x2 e2)).
-Proof. Admitted.
+Proof.
+apply_mutual_ind exp_mutind;
+default_simp.
+Qed.
 
 (* end hide *)
 
@@ -1049,7 +1305,9 @@ forall e2 e1 x1 x2,
   x1 `notin` fv_exp e2 ->
   x1 `notin` fv_exp e1 ->
   x1 `notin` fv_exp (subst_exp e1 x2 e2).
-Proof. Admitted.
+Proof.
+pose proof subst_exp_fresh_mutual as H; intuition eauto.
+Qed.
 
 Hint Resolve subst_exp_fresh : lngen.
 
@@ -1058,7 +1316,9 @@ forall e1 e2 x1,
   lc_exp e1 ->
   lc_exp e2 ->
   lc_exp (subst_exp e2 x1 e1).
-Proof. Admitted.
+Proof.
+default_simp.
+Qed.
 
 Hint Resolve subst_exp_lc_exp : lngen.
 
@@ -1068,7 +1328,10 @@ Lemma subst_exp_open_exp_wrt_exp_rec_mutual :
 (forall e3 e1 e2 x1 n1,
   lc_exp e1 ->
   subst_exp e1 x1 (open_exp_wrt_exp_rec n1 e2 e3) = open_exp_wrt_exp_rec n1 (subst_exp e1 x1 e2) (subst_exp e1 x1 e3)).
-Proof. Admitted.
+Proof.
+apply_mutual_ind exp_mutind;
+default_simp.
+Qed.
 
 (* end hide *)
 
@@ -1078,7 +1341,9 @@ Lemma subst_exp_open_exp_wrt_exp_rec :
 forall e3 e1 e2 x1 n1,
   lc_exp e1 ->
   subst_exp e1 x1 (open_exp_wrt_exp_rec n1 e2 e3) = open_exp_wrt_exp_rec n1 (subst_exp e1 x1 e2) (subst_exp e1 x1 e3).
-Proof. Admitted.
+Proof.
+pose proof subst_exp_open_exp_wrt_exp_rec_mutual as H; intuition eauto.
+Qed.
 
 Hint Resolve subst_exp_open_exp_wrt_exp_rec : lngen.
 
@@ -1088,7 +1353,9 @@ Lemma subst_exp_open_exp_wrt_exp :
 forall e3 e1 e2 x1,
   lc_exp e1 ->
   subst_exp e1 x1 (open_exp_wrt_exp e3 e2) = open_exp_wrt_exp (subst_exp e1 x1 e3) (subst_exp e1 x1 e2).
-Proof. Admitted.
+Proof.
+unfold open_exp_wrt_exp; default_simp.
+Qed.
 
 Hint Resolve subst_exp_open_exp_wrt_exp : lngen.
 
@@ -1097,7 +1364,9 @@ forall e2 e1 x1 x2,
   x1 <> x2 ->
   lc_exp e1 ->
   open_exp_wrt_exp (subst_exp e1 x1 e2) (var_f x2) = subst_exp e1 x1 (open_exp_wrt_exp e2 (var_f x2)).
-Proof. Admitted.
+Proof.
+intros; rewrite subst_exp_open_exp_wrt_exp; default_simp.
+Qed.
 
 Hint Resolve subst_exp_open_exp_wrt_exp_var : lngen.
 
@@ -1106,7 +1375,10 @@ Hint Resolve subst_exp_open_exp_wrt_exp_var : lngen.
 Lemma subst_exp_spec_rec_mutual :
 (forall e1 e2 x1 n1,
   subst_exp e2 x1 e1 = open_exp_wrt_exp_rec n1 e2 (close_exp_wrt_exp_rec n1 x1 e1)).
-Proof. Admitted.
+Proof.
+apply_mutual_ind exp_mutind;
+default_simp.
+Qed.
 
 (* end hide *)
 
@@ -1115,7 +1387,9 @@ Proof. Admitted.
 Lemma subst_exp_spec_rec :
 forall e1 e2 x1 n1,
   subst_exp e2 x1 e1 = open_exp_wrt_exp_rec n1 e2 (close_exp_wrt_exp_rec n1 x1 e1).
-Proof. Admitted.
+Proof.
+pose proof subst_exp_spec_rec_mutual as H; intuition eauto.
+Qed.
 
 Hint Resolve subst_exp_spec_rec : lngen.
 
@@ -1124,7 +1398,9 @@ Hint Resolve subst_exp_spec_rec : lngen.
 Lemma subst_exp_spec :
 forall e1 e2 x1,
   subst_exp e2 x1 e1 = open_exp_wrt_exp (close_exp_wrt_exp x1 e1) e2.
-Proof. Admitted.
+Proof.
+unfold close_exp_wrt_exp; unfold open_exp_wrt_exp; default_simp.
+Qed.
 
 Hint Resolve subst_exp_spec : lngen.
 
@@ -1135,7 +1411,10 @@ Lemma subst_exp_subst_exp_mutual :
   x2 `notin` fv_exp e2 ->
   x2 <> x1 ->
   subst_exp e2 x1 (subst_exp e3 x2 e1) = subst_exp (subst_exp e2 x1 e3) x2 (subst_exp e2 x1 e1)).
-Proof. Admitted.
+Proof.
+apply_mutual_ind exp_mutind;
+default_simp.
+Qed.
 
 (* end hide *)
 
@@ -1144,7 +1423,9 @@ forall e1 e2 e3 x2 x1,
   x2 `notin` fv_exp e2 ->
   x2 <> x1 ->
   subst_exp e2 x1 (subst_exp e3 x2 e1) = subst_exp (subst_exp e2 x1 e3) x2 (subst_exp e2 x1 e1).
-Proof. Admitted.
+Proof.
+pose proof subst_exp_subst_exp_mutual as H; intuition eauto.
+Qed.
 
 Hint Resolve subst_exp_subst_exp : lngen.
 
@@ -1157,7 +1438,10 @@ Lemma subst_exp_close_exp_wrt_exp_rec_open_exp_wrt_exp_rec_mutual :
   x2 <> x1 ->
   degree_exp_wrt_exp n1 e1 ->
   subst_exp e1 x1 e2 = close_exp_wrt_exp_rec n1 x2 (subst_exp e1 x1 (open_exp_wrt_exp_rec n1 (var_f x2) e2))).
-Proof. Admitted.
+Proof.
+apply_mutual_ind exp_mutrec;
+default_simp.
+Qed.
 
 (* end hide *)
 
@@ -1170,7 +1454,9 @@ forall e2 e1 x1 x2 n1,
   x2 <> x1 ->
   degree_exp_wrt_exp n1 e1 ->
   subst_exp e1 x1 e2 = close_exp_wrt_exp_rec n1 x2 (subst_exp e1 x1 (open_exp_wrt_exp_rec n1 (var_f x2) e2)).
-Proof. Admitted.
+Proof.
+pose proof subst_exp_close_exp_wrt_exp_rec_open_exp_wrt_exp_rec_mutual as H; intuition eauto.
+Qed.
 
 Hint Resolve subst_exp_close_exp_wrt_exp_rec_open_exp_wrt_exp_rec : lngen.
 
@@ -1183,16 +1469,20 @@ forall e2 e1 x1 x2,
   x2 <> x1 ->
   lc_exp e1 ->
   subst_exp e1 x1 e2 = close_exp_wrt_exp x2 (subst_exp e1 x1 (open_exp_wrt_exp e2 (var_f x2))).
-Proof. Admitted.
+Proof.
+unfold close_exp_wrt_exp; unfold open_exp_wrt_exp; default_simp.
+Qed.
 
 Hint Resolve subst_exp_close_exp_wrt_exp_open_exp_wrt_exp : lngen.
 
 Lemma subst_exp_abs :
-forall x2 T1 e2 e1 x1,
+forall x2 e2 e1 x1,
   lc_exp e1 ->
   x2 `notin` fv_exp e1 `union` fv_exp e2 `union` singleton x1 ->
-  subst_exp e1 x1 (abs T1 e2) = abs (T1) (close_exp_wrt_exp x2 (subst_exp e1 x1 (open_exp_wrt_exp e2 (var_f x2)))).
-Proof. Admitted.
+  subst_exp e1 x1 (abs e2) = abs (close_exp_wrt_exp x2 (subst_exp e1 x1 (open_exp_wrt_exp e2 (var_f x2)))).
+Proof.
+default_simp.
+Qed.
 
 Hint Resolve subst_exp_abs : lngen.
 
@@ -1202,7 +1492,10 @@ Lemma subst_exp_intro_rec_mutual :
 (forall e1 x1 e2 n1,
   x1 `notin` fv_exp e1 ->
   open_exp_wrt_exp_rec n1 e2 e1 = subst_exp e2 x1 (open_exp_wrt_exp_rec n1 (var_f x1) e1)).
-Proof. Admitted.
+Proof.
+apply_mutual_ind exp_mutind;
+default_simp.
+Qed.
 
 (* end hide *)
 
@@ -1210,7 +1503,9 @@ Lemma subst_exp_intro_rec :
 forall e1 x1 e2 n1,
   x1 `notin` fv_exp e1 ->
   open_exp_wrt_exp_rec n1 e2 e1 = subst_exp e2 x1 (open_exp_wrt_exp_rec n1 (var_f x1) e1).
-Proof. Admitted.
+Proof.
+pose proof subst_exp_intro_rec_mutual as H; intuition eauto.
+Qed.
 
 Hint Resolve subst_exp_intro_rec : lngen.
 Hint Rewrite subst_exp_intro_rec using solve [auto] : lngen.
@@ -1219,7 +1514,9 @@ Lemma subst_exp_intro :
 forall x1 e1 e2,
   x1 `notin` fv_exp e1 ->
   open_exp_wrt_exp e1 e2 = subst_exp e2 x1 (open_exp_wrt_exp e1 (var_f x1)).
-Proof. Admitted.
+Proof.
+unfold open_exp_wrt_exp; default_simp.
+Qed.
 
 Hint Resolve subst_exp_intro : lngen.
 
